

Double Pendulum - Equations of Motion

Miruna and Venus

February 2026

1. System Description

We consider a double pendulum consisting of:

- Masses: m_1, m_2
- Massless rod lengths: ℓ_1, ℓ_2
- Angles from vertical: $\theta_1(t), \theta_2(t)$

2. Coordinates

Mass 1

$$x_1 = \ell_1 \sin \theta_1 \tag{1}$$

$$y_1 = -\ell_1 \cos \theta_1 \tag{2}$$

Mass 2

$$x_2 = \ell_1 \sin \theta_1 + \ell_2 \sin \theta_2 \tag{3}$$

$$y_2 = -\ell_1 \cos \theta_1 - \ell_2 \cos \theta_2 \tag{4}$$

3. Velocities

Mass 1

$$\dot{x}_1 = \ell_1 \cos \theta_1 \dot{\theta}_1$$

$$\dot{y}_1 = \ell_1 \sin \theta_1 \dot{\theta}_1$$

The squared velocity becomes:

$$v_1^2 = \dot{x}_1^2 + \dot{y}_1^2$$

$$\boxed{v_1^2 = \ell_1^2 \dot{\theta}_1^2} \tag{5}$$

Mass 2

$$\begin{aligned}\dot{x}_2 &= \ell_1 \cos \theta_1 \dot{\theta}_1 + \ell_2 \cos \theta_2 \dot{\theta}_2 \\ \dot{y}_2 &= \ell_1 \sin \theta_1 \dot{\theta}_1 + \ell_2 \sin \theta_2 \dot{\theta}_2\end{aligned}$$

The squared velocity becomes:

$$v_2^2 = \dot{x}_2^2 + \dot{y}_2^2$$

$$\boxed{v_2^2 = \ell_1^2 \dot{\theta}_1^2 + \ell_2^2 \dot{\theta}_2^2 + 2\ell_1 \ell_2 \dot{\theta}_1 \dot{\theta}_2 \cos(\theta_1 - \theta_2)} \quad (6)$$

4. Kinetic Energy

$$T = \frac{1}{2}m_1 v_1^2 + \frac{1}{2}m_2 v_2^2$$

Substituting:

$$T = \frac{1}{2}m_1 \ell_1^2 \dot{\theta}_1^2 + \frac{1}{2}m_2 \left(\ell_1^2 \dot{\theta}_1^2 + \ell_2^2 \dot{\theta}_2^2 + 2\ell_1 \ell_2 \dot{\theta}_1 \dot{\theta}_2 \cos(\theta_1 - \theta_2) \right)$$

Rearranged:

$$\boxed{T = \frac{1}{2}(m_1 + m_2)\ell_1^2 \dot{\theta}_1^2 + \frac{1}{2}m_2 \ell_2^2 \dot{\theta}_2^2 + m_2 \ell_1 \ell_2 \dot{\theta}_1 \dot{\theta}_2 \cos(\theta_1 - \theta_2)} \quad (7)$$

5. Potential Energy

$$V = m_1 g y_1 + m_2 g y_2$$

Substituting:

$$\boxed{V = -(m_1 + m_2)g\ell_1 \cos \theta_1 - m_2 g \ell_2 \cos \theta_2} \quad (8)$$

6. The Lagrangian

$$L = T - V$$

$$\boxed{L = \frac{1}{2}(m_1 + m_2)\ell_1^2 \dot{\theta}_1^2 + \frac{1}{2}m_2 \ell_2^2 \dot{\theta}_2^2 + m_2 \ell_1 \ell_2 \dot{\theta}_1 \dot{\theta}_2 \cos(\theta_1 - \theta_2) + (m_1 + m_2)g\ell_1 \cos \theta_1 + m_2 g \ell_2 \cos \theta_2} \quad (9)$$

7. Euler–Lagrange Equations

For each coordinate:

$$\boxed{\frac{d}{dt} \left(\frac{\partial L}{\partial \dot{\theta}_i} \right) - \frac{\partial L}{\partial \theta_i} = 0} \quad (10)$$

8. Equation for θ_1

After computing derivatives and simplifying:

$$(m_1 + m_2)\ell_1\ddot{\theta}_1 + m_2\ell_2\ddot{\theta}_2 \cos(\theta_1 - \theta_2) + m_2\ell_2\dot{\theta}_2^2 \sin(\theta_1 - \theta_2) + (m_1 + m_2)g \sin \theta_1 = 0$$

9. Equation for θ_2

$$\ell_2\ddot{\theta}_2 + \ell_1\ddot{\theta}_1 \cos(\theta_1 - \theta_2) - \ell_1\dot{\theta}_1^2 \sin(\theta_1 - \theta_2) + g \sin \theta_2 = 0$$

10. Equations of Motion for the Double Pendulum

$$\boxed{\ddot{\theta}_1 = \frac{-g(2m_1 + m_2) \sin \theta_1 - m_2 g \sin(\theta_1 - 2\theta_2) - 2 \sin(\theta_1 - \theta_2) m_2 (\dot{\theta}_2^2 \ell_2 + \dot{\theta}_1^2 \ell_1 \cos(\theta_1 - \theta_2))}{\ell_1 (2m_1 + m_2 - m_2 \cos(2(\theta_1 - \theta_2)))}} \quad (11)$$

$$\boxed{\ddot{\theta}_2 = \frac{2 \sin(\theta_1 - \theta_2) \left(\dot{\theta}_1^2 \ell_1 (m_1 + m_2) + g(m_1 + m_2) \cos \theta_1 + \dot{\theta}_2^2 \ell_2 m_2 \cos(\theta_1 - \theta_2) \right)}{\ell_2 (2m_1 + m_2 - m_2 \cos(2(\theta_1 - \theta_2)))}} \quad (12)$$